Update notations so we no longer have notation conflicts.

coq-osiris/examples/proofs/iter.v
@@ -18,17 +18,17 @@ Definition isListIter (iter : val) : iProp Σ :=
     □ (∀ (Xs : list A) (X : A),
           ⌜ (Xs ++ [X]) `prefix_of` l ⌝ -∗
             I Xs -∗
-            EWP (call f #X) @ E <| ψ |> {{ | RET v => ⌜ v = VUnit ⌝ ∗ I (Xs ++ [X]);
+            EWP (call f #X) @ E <| ψ |> {{   RET v => ⌜ v = VUnit ⌝ ∗ I (Xs ++ [X]);
                                            | EXN e => φ e ∗ I Xs }})
       -∗
       I [] -∗
       EWP (ncall iter [f; #l] ) @E <| ψ |>
-      {{ | RET v => ⌜ v = VUnit ⌝ ∗ I l;
+      {{   RET v => ⌜ v = VUnit ⌝ ∗ I l;
          | EXN e => φ e ∗ ∃ Xs, I Xs ∗ ⌜ Xs `prefix_of` l ⌝ }}.
 
 Lemma iter_module :
   ⊢ EWP (eval_mexpr stdlib_env __main)
-    {{ RET m, module_spec [("iter", isListIter)] m}}.
+    {{ ensures m, module_spec [("iter", isListIter)] m}}.
 Proof.
   iIntros. unfold __main.
   iApply ewp_module.
