coq-osiris/theories/proofmode/proofmode.v
@@ -2,7 +2,6 @@ From osiris.proofmode Require Export
   equality
   pure_tactics
   ewp_tactics
-  notations
   specifications
 .
 (* [setup.v] should be exported last. *)
